PyLevelLang/src/PyLevelLang/Interpret.v
@@ -43,7 +43,7 @@ Fixpoint eval_range_word (lo : word) (len : nat) : list word :=
   | S n => lo :: eval_range_word (word.add lo (word.of_Z 1)) n
   end.
 
-Definition proj_expected (t_expected : type) (v : {t_actual & interp_type t_actual}) : 
+Definition proj_expected (t_expected : type) (v : {t_actual & interp_type t_actual}) :
   interp_type t_expected :=
   match type_eq_dec (projT1 v) t_expected with
   | left H => cast H _ (projT2 v)
@@ -99,10 +99,10 @@ Section WithMap.
     | OIntToString => fun n => DecimalString.NilZero.string_of_int (BinInt.Z.to_int n)
     end.
 
-  Definition interp_binop {t1 t2 t3: type} (o : binop t1 t2 t3) : 
-    interp_type t1 -> interp_type t2 -> interp_type t3 := 
-    match o in binop t1 t2 t3 
-    return interp_type t1 -> interp_type t2 -> interp_type t3 with 
+  Definition interp_binop {t1 t2 t3: type} (o : binop t1 t2 t3) :
+    interp_type t1 -> interp_type t2 -> interp_type t3 :=
+    match o in binop t1 t2 t3
+    return interp_type t1 -> interp_type t2 -> interp_type t3 with
     | OWPlus => word.add
     | OPlus =>  Z.add
     | OWMinus => word.sub
@@ -130,31 +130,38 @@ Section WithMap.
     | OWRange => fun s e => eval_range_word s (Z.to_nat (word.unsigned e - word.unsigned s))
     end.
 
-  Fixpoint interp_expr (l : locals) {t : type} (e : expr t) : interp_type t :=
-    match e in (expr t0) return (interp_type t0) with
-    | EVar _ x | ELoc _ x => get_local l x
+   Fixpoint interp_expr (store env : locals) {t : type} (e : expr t) : interp_type t :=
+    match e with
+    | EVar _ x => get_local env x
+    | ELoc _ x => get_local store x
     | EAtom a => interp_atom a
-    | EUnop o e1 => interp_unop o (interp_expr l e1)
-    | EBinop o e1 e2 => interp_binop o (interp_expr l e1) (interp_expr l e2)
-    | EFlatmap l1 x fn => flat_map (fun y => interp_expr (set_local l x y) fn) (interp_expr l l1)
-    | EIf e1 e2 e3 => if interp_expr l e1 then interp_expr l e2 else interp_expr l e3
-    | EFold l1 a x y fn => let l1' := interp_expr l l1 in
-                             let a' := interp_expr l a in
-                             let fn' := fun v acc => interp_expr (set_local (set_local l x v) y acc) fn in
-                             fold_right fn' a' l1'
-    | ELet x e1 e2 => interp_expr (set_local l x (interp_expr l e1)) e2
+    | EUnop o e1 => interp_unop o (interp_expr store env e1)
+    | EBinop o e1 e2 => interp_binop o (interp_expr store env  e1) (interp_expr store env  e2)
+    | EFlatmap l1 x fn => flat_map (fun y => interp_expr store (set_local env x y) fn) (interp_expr store env  l1)
+    | EIf e1 e2 e3 => if interp_expr store env e1 then interp_expr store env e2 else interp_expr store env e3
+    | EFold l1 a x y fn => let l1' := interp_expr store env l1 in
+                           let a' := interp_expr store env a in
+                           let fn' := fun v acc => interp_expr store (set_local (set_local env x v) y acc) fn in
+                           fold_right fn' a' l1'
+    | ELet x e1 e2 => interp_expr store (set_local env x (interp_expr store env e1)) e2
     end.
 
-  Fixpoint interp_command (l : locals) (c : command) : locals :=
+  Fixpoint interp_command (store env : locals) (c : command) : locals :=
     match c with
-    | CSkip => l
-    | CSeq c1 c2 => interp_command (interp_command l c1) c2
-    | CLet x e c1 | CLetMut x e c1 => let l' := interp_command (set_local l x (interp_expr l e)) c1 in
-                                      map.update l' x (map.get l x)
-    | CGets x e => set_local l x (interp_expr l e)
-    | CIf e c1 c2 => if interp_expr l e then interp_command l c1 else interp_command l c2
-    | CForeach x e c1 => let l' := fold_left (fun l' v => interp_command (set_local l' x v) c1) (interp_expr l e) l in
-                         map.update l' x (map.get l x)
+    | CSkip => store
+    | CSeq c1 c2 =>
+        let store' := interp_command store env c1 in
+        interp_command store' env c2
+    | CLet x e c1 =>
+        let env' := set_local env x (interp_expr store env e) in
+        interp_command store env' c1
+    | CLetMut x e c1 =>
+        let store' := set_local store x (interp_expr store env e) in
+        let store'' := interp_command store' env c1 in
+        map.update store'' x (map.get store x)
+    | CGets x e => set_local store x (interp_expr store env e)
+    | CIf e c1 c2 => if interp_expr store env e then interp_command store env c1 else interp_command store env c2
+    | CForeach x e c1 => fold_left (fun store' v => interp_command store' (set_local env x v) c1) (interp_expr store env e) store
     end.
 End WithMap.
 End WithWord.
