PyLevelLang/src/PyLevelLang/Phoas_Interpret.v
@@ -5,31 +5,81 @@ Require Import PyLevelLang.Elaborate.
 Require Import Coq.Strings.String.
 Require Import Coq.Logic.FunctionalExtensionality.
 
+Section PhoasExprEquiv.
+  Context {V V' : type -> Type}.
+
+  Definition ctxt := list { t : type & (V t * V' t)%type }.
+  Definition vars := existT (fun t => (V t * V' t)%type).
+
+  Inductive phoas_expr_equiv : ctxt -> forall {t : type},
+        phoas_expr V t -> phoas_expr V' t -> Prop :=
+  | eq_PhEVar C t (v : V t) (v' : V' t) :
+    In (vars _ (v, v')) C -> phoas_expr_equiv C (PhEVar _ v) (PhEVar _ v')
+  | eq_PhELoc C t (x x' : string) :
+    x = x' -> phoas_expr_equiv C (PhELoc t x) (PhELoc t x')
+  | eq_PhEAtom C {t} (a a' : atom t) :
+    a = a' -> phoas_expr_equiv C (PhEAtom a) (PhEAtom a')
+  | eq_PhEUnop C {t1 t2} (o : unop t1 t2) e e' :
+    phoas_expr_equiv C e e' ->
+    phoas_expr_equiv C (PhEUnop o e) (PhEUnop o e')
+  | eq_PhEBinop C {t1 t2 t3} (o : binop t1 t2 t3) e1 e1' e2 e2' :
+    phoas_expr_equiv C e1 e1' ->
+    phoas_expr_equiv C e2 e2' ->
+    phoas_expr_equiv C (PhEBinop o e1 e2) (PhEBinop o e1' e2')
+  | eq_PhEFlatmap C {t1 t2} l1 l1' (x x' : string) (fn_l2 : V t1 -> phoas_expr V (TList t2)) fn_l2':
+    phoas_expr_equiv C l1 l1' ->
+    (forall v v', phoas_expr_equiv (vars _ (v, v') :: C) (fn_l2 v) (fn_l2' v')) ->
+    phoas_expr_equiv C (PhEFlatmap l1 x fn_l2) (PhEFlatmap l1' x' fn_l2')
+  | eq_PhEFold C {t1 t2} l1 l1' e2 e2' (x x' y y' : string) (fn_e3 : V t1 -> V t2 -> phoas_expr V t2) fn_e3' :
+    phoas_expr_equiv C l1 l1' ->
+    phoas_expr_equiv C e2 e2' ->
+    (forall v1 v2 v1' v2', phoas_expr_equiv (vars _ (v2, v2') :: vars _ (v1, v1') :: C) (fn_e3 v1 v2) (fn_e3' v1' v2')) ->
+    phoas_expr_equiv C (PhEFold l1 e2 x y fn_e3) (PhEFold l1' e2' x' y' fn_e3')
+  | eq_PhEIf C {t} e1 e1' (e2 : phoas_expr V t) e2' e3 e3' :
+    phoas_expr_equiv C e1 e1' ->
+    phoas_expr_equiv C e2 e2' ->
+    phoas_expr_equiv C e3 e3' ->
+    phoas_expr_equiv C (PhEIf e1 e2 e3) (PhEIf e1' e2' e3')
+  | eq_PhELet C {t1 t2} (x x' : string) e1 e1' (fn_e2 : V t1 -> phoas_expr V t2) fn_e2' :
+    phoas_expr_equiv C e1 e1' ->
+    (forall v v', phoas_expr_equiv (vars _ (v, v') :: C) (fn_e2 v) (fn_e2' v')) ->
+    phoas_expr_equiv C (PhELet x e1 fn_e2) (PhELet x' e1' fn_e2').
+End PhoasExprEquiv.
+
+Definition projT1_fst_T2 {A : Type} {P1 P2 : A -> Type} (v : {t : A & (P1 t * P2 t)%type}) :
+  {t : A & P1 t} :=
+  existT _ (projT1 v) (fst (projT2 v)).
+
+Definition projT1_snd_T2 {A : Type} {P1 P2 : A -> Type} (v : {t : A & (P1 t * P2 t)%type}) :
+  {t : A & P2 t} :=
+  existT _ (projT1 v) (snd (projT2 v)).
+
 Section WithMap.
   Context {width: Z} {BW: Bitwidth width} {word: word.word width} {mem: map.map word byte}.
   Context {word_ok: word.ok word} {mem_ok: map.ok mem}.
-  Context {locals: map.map string {t & interp_type (width := width) t}} {locals_ok: map.ok locals}.
+  Context {phoas_env : forall V, map.map string {t : type & V t}} {phoas_env_ok : forall V, map.ok (phoas_env V)}.
 
-
-  Fixpoint interp_phoas_expr {t : type} (l : locals) (e : phoas_expr interp_type t) : interp_type t :=
+  Fixpoint interp_phoas_expr {t : type} (store : phoas_env interp_type) (e : phoas_expr interp_type t) : interp_type t :=
     match e with
     | PhEVar _ v => v
-    | PhELoc _ x => get_local l x
+    | PhELoc _ x => get_local store x
     | PhEAtom a => interp_atom a
-    | PhEUnop o e1 => interp_unop o (interp_phoas_expr l e1)
-    | PhEBinop o e1 e2 => interp_binop o (interp_phoas_expr l e1) (interp_phoas_expr l e2)
-    | PhEFlatmap l1 _ fn_l2 => flat_map (fun y => interp_phoas_expr l (fn_l2 y)) (interp_phoas_expr l l1)
-    | PhEFold l1 e2 _ _ fn_e3 => let l1' := interp_phoas_expr l l1 in
-                                 let a' := interp_phoas_expr l e2 in
-                                 let fn' := fun v acc => interp_phoas_expr l (fn_e3 v acc) in
+    | PhEUnop o e1 => interp_unop o (interp_phoas_expr store e1)
+    | PhEBinop o e1 e2 => interp_binop o (interp_phoas_expr store e1) (interp_phoas_expr store e2)
+    | PhEFlatmap l1 _ fn_l2 => flat_map (fun y => interp_phoas_expr store (fn_l2 y)) (interp_phoas_expr store l1)
+    | PhEFold l1 e2 _ _ fn_e3 => let l1' := interp_phoas_expr store l1 in
+                                 let a' := interp_phoas_expr store e2 in
+                                 let fn' := fun v acc => interp_phoas_expr store (fn_e3 v acc) in
                                  fold_right fn' a' l1'
-    | PhEIf e1 e2 e3 => if interp_phoas_expr l e1 then interp_phoas_expr l e2 else interp_phoas_expr l e3
-    | PhELet _ e1 fn_e2 => interp_phoas_expr l (fn_e2 (interp_phoas_expr l e1))
+    | PhEIf e1 e2 e3 => if interp_phoas_expr store e1 then interp_phoas_expr store e2 else interp_phoas_expr store e3
+    | PhELet _ e1 fn_e2 => interp_phoas_expr store (fn_e2 (interp_phoas_expr store e1))
     end.
 
-  Section WithPhoasMap.
+  Definition interp_Phoas_expr (store : phoas_env interp_type) {t : type} (e : Phoas_expr t) :=
+    interp_phoas_expr store (e _).
+
+  Section WithPhoasV.
     Context {V : type -> Type}.
-    Context {phoas_env: map.map string {t & V t}} {phoas_env_ok: map.ok phoas_env}.
 
     (* Default value of type (phoas_expr V t) *)
     Fixpoint default_phoas_expr (t : type) : phoas_expr V t :=
@@ -53,10 +103,10 @@ Section WithMap.
       | _ => default_phoas_expr t_expected
       end.
 
-    Definition set_phoas_local (env : phoas_env) (x : string) {t : type} (v : V t) :=
+    Definition set_phoas_local (env : phoas_env V) (x : string) {t : type} (v : V t) :=
       map.put env x (existT _ _ v).
 
-    Fixpoint phoasify {t : type} (env : phoas_env) (e : expr t) : phoas_expr V t :=
+    Fixpoint phoasify (env : phoas_env V) {t : type} (e : expr t) : phoas_expr V t :=
       match e with
       | EVar _ x => match map.get env x with
                     | Some v => phoas_proj_expected _ v
@@ -73,471 +123,374 @@ Section WithMap.
                                (fun v acc => phoasify (set_phoas_local (set_phoas_local env x v) y acc) fn)
       | ELet x e1 e2 => PhELet x (phoasify env e1) (fun v => phoasify (set_phoas_local env x v) e2)
       end.
-  End WithPhoasMap.
+  End WithPhoasV.
 
-  (* Remove one occurrence of x from l if there is one.
-   * Auxiliary function for the definition of fresh' below *)
-  Fixpoint remove_one (x : string) (l : list string) : list string :=
-    match l with
-    | nil => nil
-    | h :: t => if eqb h x then t else h :: remove_one x t
-    end.
-
-  Lemma in_remove_one_len : forall (x : string) (l : list string),
-      In x l -> List.length l = S (List.length (remove_one x l)).
-  Proof.
-    intros. induction l.
-    - apply in_nil in H. exfalso. apply H.
-    - simpl in H. destruct (eqb a x) eqn:E.
-      + simpl. rewrite E. reflexivity.
-      + destruct H as [HL | HR].
-        * rewrite <- eqb_eq in HL. rewrite HL in E. discriminate.
-        * simpl. rewrite E. simpl. rewrite (IHl HR). reflexivity.
-  Qed.
-
-  Lemma in_remove_one : forall (x : string) (l : list string),
-      In x l -> forall (y : string), x = y \/ In x (remove_one y l).
-  Proof.
-    intros x l H. induction l.
-    - intros. apply in_nil in H. exfalso. exact H.
-    - intros y. simpl in H. destruct H as [HL | HR].
-      + destruct (eqb a y) eqn:E.
-        * rewrite eqb_eq in E. rewrite HL in E. left. exact E.
-        * right. simpl. rewrite E. simpl. left. exact HL.
-      + destruct (IHl HR) with (y := y) as [HL' | HR'].
-        * left. exact HL'.
-        * right. simpl. destruct (eqb a y) eqn:E.
-          { exact HR. }
-          { simpl. right. exact HR'. }
-  Qed.
-
-  (* Append "'"s to x until the resulting name is not in used.
-   * The initial call should have (budget = length used) *)
-  Fixpoint fresh' (budget : nat) (used : list string) (x : string) : string :=
-    (* We need budget as a decreasing argument for the function *)
-    match budget with
-    | O => x
-    | S n => match in_dec string_dec x used with
-             | left _ => fresh' n (remove_one x used) (x ++ "'")
-             | right _ => x
-             end
-    end.
-
-  (* Given a list of used names and a hint, return a fresh name *)
-  Definition fresh (used : list string) (x : string) : string :=
-    fresh' (List.length used) used x.
-
-  Lemma len_app : forall y, length y < length (y ++ "'").
-  Proof.
-    induction y; auto. simpl. apply Arith_prebase.lt_n_S_stt. apply IHy.
-  Qed.
-
-  Lemma fresh'_len : forall (budget : nat) (used : list string) (x : string),
-      length x <= length (fresh' budget used x).
-  Proof.
-    induction budget; intros.
-    - destruct used; unfold fresh'; constructor.
-    - destruct (in_dec string_dec x used) eqn:E.
-      + unfold fresh'. rewrite E.
-        apply Nat.le_trans with (m := length (x ++ "'")).
-        * pose proof (len_app x) as len_app_x.
-          apply Nat.lt_le_incl. exact len_app_x.
-        * apply (IHbudget (remove_one x used) (x ++ "'")%string).
-      + unfold fresh'; rewrite E; constructor.
-  Qed.
-
-  Lemma fresh'_is_fresh : forall (budget : nat) (used : list string) (x : string),
-      budget = List.length used -> ~ In (fresh' budget used x) used.
-  Proof.
-    induction budget; intros.
-    - destruct used.
-      + auto.
-      + discriminate.
-    - rewrite H. destruct (in_dec string_dec x used) as [ HL | HR ] eqn:E.
-      + assert (Hrm_len: S budget = S (List.length (remove_one x used))).
-        { rewrite H. apply in_remove_one_len. apply HL. }
-        injection Hrm_len as Hrm_len.
-        apply (IHbudget (remove_one x used)) with (x := (x ++ "'")%string) in Hrm_len as Hrm.
-        unfold not. intros. apply in_remove_one with (y := x) in H0 as [HL'|HR'].
-        * assert (HA : length (x ++ "'") <= length (fresh' (Datatypes.length used) used x)).
-          { unfold fresh'. rewrite <- H. rewrite E. apply fresh'_len. }
-          rewrite HL' in HA. apply Arith_prebase.le_not_lt_stt in HA.
-          apply HA. apply len_app.
-        * unfold fresh' in HR'. rewrite <- H in HR'. rewrite E in HR'.
-          apply Hrm. unfold fresh'. apply HR'.
-      + unfold fresh'. rewrite <- H. rewrite E. exact HR.
-  Qed.
-
-  Corollary fresh_is_fresh : forall (used : list string) (x : string), ~ In (fresh used x) used.
-  Proof.
-    intros. unfold fresh. apply fresh'_is_fresh. reflexivity.
-  Qed.
-
-  Definition const_string : type -> Type := fun _ => string.
-
-  Fixpoint dephoasify (used : list string) {t : type} (e : phoas_expr const_string t) : expr t :=
-    match e with
-    | PhEVar _ v => EVar _ v
-    | PhELoc _ x => ELoc _ x
-    | PhEAtom a => EAtom a
-    | PhEUnop o e1 => EUnop o (dephoasify used e1)
-    | PhEBinop o e1 e2 => EBinop o (dephoasify used e1) (dephoasify used e2)
-    | PhEFlatmap l1 x fn =>
-        let x' := fresh used x in
-        let used' := x' :: used in
-        EFlatmap (dephoasify used' l1) x' (dephoasify used' (fn x'))
-    | PhEIf e1 e2 e3 => EIf (dephoasify used e1) (dephoasify used e2) (dephoasify used e3)
-    | PhEFold l1 a x y fn =>
-        let x' := fresh used x in
-        let y' := fresh (x' :: used) y in
-        let used' := y' :: x' :: used in
-        EFold (dephoasify used l1) (dephoasify used a) x' y' (dephoasify used' (fn x' y'))
-    | PhELet x e1 fn =>
-        let x' := fresh used x in
-        let used' := x' :: used in
-        ELet x' (dephoasify used e1) (dephoasify used' (fn x'))
-    end.
-
-  Context {tenv : map.map string (type * bool)} {tenv_ok : map.ok tenv}.
-
-  Lemma eq_dec_refl : forall  {t : Type} (eq_dec : forall (v1 v2 : t), {v1 = v2} + {v1 <> v2}),
-    forall (x : t), eq_dec x x = left eq_refl.
-  Proof.
-    intros t eq_dec x. destruct (eq_dec x x).
-    - f_equal. apply Eqdep_dec.UIP_dec. apply eq_dec.
-    - exfalso. apply n. reflexivity.
-  Qed.
-
-  Ltac eq_projT2_eq := match goal with
-                       | H : existT ?f ?t _ = existT ?f ?t _ |- _ =>
-                           apply Eqdep_dec.inj_pair2_eq_dec in H;[ subst; eauto | apply type_eq_dec]
-                       end.
-
-  Section WithPhoasEnv.
-    Context {phoas_env : forall V, map.map string {t : type & V t}} {phoas_env_ok : forall V, map.ok (phoas_env V)}.
-
-    Definition phoasify_envs_consistent (G : tenv) (l : locals) (env : phoas_env interp_type) (store : locals) : Prop :=
-      forall x,
-        match map.get G x, map.get l x with
-        | Some (t, is_mut), Some v =>
-            if is_mut then map.get store x = Some v  /\ projT1 v = t
-            else  map.get env x = Some v  /\ projT1 v = t
-        | Some _, None => False
-        | None, _ => True
-        end.
-
-    Lemma phoasify_envs_consistent_immut_step : forall G l env store x t (v : interp_type t), phoasify_envs_consistent G l env store -> phoasify_envs_consistent (map.put G x (t, false)) (set_local l x v) (set_phoas_local env x v) store.
-    Proof.
-      unfold phoasify_envs_consistent. intros. unfold set_local. unfold set_phoas_local. destruct (string_dec x0 x).
-      - subst. repeat rewrite map.get_put_same; eauto.
-      - repeat rewrite map.get_put_diff by assumption. pose proof (H x0) as H0.
-        destruct (map.get G x0) eqn:E; auto.
-    Qed.
-
-    Lemma phoasify_sound' :
-      forall {t : type} (e : expr t) (G : tenv),
-        wf G e ->
-        forall (l : locals) (env : phoas_env interp_type) (store : locals),
-          phoasify_envs_consistent G l env store ->
-          interp_expr l e = interp_phoas_expr store (phoasify env e).
-    Proof.
-      induction e; intros; simpl.
-      - unfold get_local. inversion H. unfold phoasify_envs_consistent in H0.
-        pose proof (H0 x) as Hx. rewrite H4 in Hx. unfold phoas_proj_expected.
-        destruct (map.get l x).
-        + destruct Hx. unfold proj_expected. subst. rewrite H5.
-          rewrite (eq_dec_refl type_eq_dec). reflexivity.
-        + exfalso. exact Hx.
-      - unfold get_local. inversion H. unfold phoasify_envs_consistent in H0.
-        pose proof (H0 x) as Hx. rewrite H4 in Hx. unfold phoas_proj_expected.
-        destruct (map.get l x).
-        + destruct  Hx. unfold proj_expected. subst. rewrite H5.
-          rewrite (eq_dec_refl type_eq_dec). reflexivity.
-        + exfalso. exact Hx.
-      - reflexivity.
-      - f_equal. inversion H. eq_projT2_eq.
-      - inversion H; subst; repeat eq_projT2_eq. f_equal; eauto.
-      - inversion H; repeat eq_projT2_eq. f_equal.
-        + extensionality y. apply (IHe2 _ H8). apply phoasify_envs_consistent_immut_step. assumption.
-        + eapply (IHe1 G); assumption.
-      - inversion H; repeat eq_projT2_eq. f_equal.
-        + extensionality v. extensionality acc. apply (IHe3 _ H11).
-          repeat apply phoasify_envs_consistent_immut_step. assumption.
-        + apply (IHe2 G); assumption.
-        + apply (IHe1 G); assumption.
-      - inversion H; repeat eq_projT2_eq. destruct (interp_expr l e1) eqn:E;
-          rewrite (IHe1 _ H6 _ _ _ H0) in E; rewrite E.
-        + apply (IHe2 _ H7 _ _ _ H0).
-        + apply (IHe3 _ H8 _ _ _ H0).
-      - inversion H; repeat eq_projT2_eq.
-        rewrite (IHe1 _ H5 _ _ _ H0).
-        apply (IHe2 _ H8). apply phoasify_envs_consistent_immut_step. exact H0.
-    Qed.
-
-    Definition Phoasify {t : type} (e : expr t) : Phoas_expr t:=
-      fun (V : type -> Type) => phoasify (V := V) map.empty e.
-
-    Definition phoasify_envs_consistent_closed (G : tenv) (l store : locals) : Prop :=
-      forall x, match map.get G x with
-                | Some (t, true) =>
-                    match map.get l x with
-                    | Some v => map.get store x = Some v /\ projT1 v = t
-                    | None => False
-                    end
-                | _ => True
-                end.
-
-    Definition Flat_wf (G : tenv) {t : type} (e : expr t) :=
-      (forall x, match map.get G x with
-                 | Some (t, is_mut) =>
-                     (* All variables are mutable *)
-                     is_mut = true
-                 | None => True
-                 end) /\
-        wf G e.
-
-    Theorem phoasify_sound : forall {t : type} (e : expr t) (G : tenv),
-        Flat_wf G e ->
-        forall l store : locals,
-          phoasify_envs_consistent_closed G l store ->
-          interp_expr l e = interp_phoas_expr store (Phoasify e interp_type).
-    Proof.
-      intros t e G [H_closed H_wf] l store H_consistent_closed.
-      assert (H_consistent : phoasify_envs_consistent G l map.empty store).
-      { unfold phoasify_envs_consistent. intro x.
-        pose proof (H_closed x) as H_closed'.
-        pose proof (H_consistent_closed x) as H_consistent_closed'.
-        destruct (map.get G x) eqn:E; trivial. destruct p. subst.
-        assumption.
-      }
-      unfold Phoasify. eapply phoasify_sound'.
-      - apply H_wf.
-      - assumption.
-    Qed.
-  End WithPhoasEnv.
-
-  Section expr_equiv.
-    Context {V V' : type -> Type}.
-
-    Definition ctxt := list { t : type & (V t * V' t)%type }.
-    Definition vars := existT (fun t => (V t * V' t)%type).
-
-    Inductive phoas_expr_equiv : ctxt -> forall {t : type},
-          phoas_expr V t -> phoas_expr V' t -> Prop :=
-    | eq_PhEVar C t (v : V t) (v' : V' t) :
-      In (vars _ (v, v')) C -> phoas_expr_equiv C (PhEVar _ v) (PhEVar _ v')
-    | eq_PhELoc C t (x x' : string) :
-      x = x' -> phoas_expr_equiv C (PhELoc t x) (PhELoc t x')
-    | eq_PhEAtom C {t} (a a' : atom t) :
-      a = a' -> phoas_expr_equiv C (PhEAtom a) (PhEAtom a')
-    | eq_PhEUnop C {t1 t2} (o : unop t1 t2) e e' :
-      phoas_expr_equiv C e e' ->
-      phoas_expr_equiv C (PhEUnop o e) (PhEUnop o e')
-    | eq_PhEBinop C {t1 t2 t3} (o : binop t1 t2 t3) e1 e1' e2 e2' :
-      phoas_expr_equiv C e1 e1' ->
-      phoas_expr_equiv C e2 e2' ->
-      phoas_expr_equiv C (PhEBinop o e1 e2) (PhEBinop o e1' e2')
-    | eq_PhEFlatmap C {t1 t2} l1 l1' (x x' : string) (fn_l2 : V t1 -> phoas_expr V (TList t2)) fn_l2':
-      phoas_expr_equiv C l1 l1' ->
-      (forall v v', phoas_expr_equiv (vars _ (v, v') :: C) (fn_l2 v) (fn_l2' v')) ->
-      phoas_expr_equiv C (PhEFlatmap l1 x fn_l2) (PhEFlatmap l1' x' fn_l2')
-    | eq_PhEFold C {t1 t2} l1 l1' e2 e2' (x x' y y' : string) (fn_e3 : V t1 -> V t2 -> phoas_expr V t2) fn_e3' :
-      phoas_expr_equiv C l1 l1' ->
-      phoas_expr_equiv C e2 e2' ->
-      (forall v1 v2 v1' v2', phoas_expr_equiv (vars _ (v2, v2') :: vars _ (v1, v1') :: C) (fn_e3 v1 v2) (fn_e3' v1' v2')) ->
-      phoas_expr_equiv C (PhEFold l1 e2 x y fn_e3) (PhEFold l1' e2' x' y' fn_e3')
-    | eq_PhEIf C {t} e1 e1' (e2 : phoas_expr V t) e2' e3 e3' :
-      phoas_expr_equiv C e1 e1' ->
-      phoas_expr_equiv C e2 e2' ->
-      phoas_expr_equiv C e3 e3' ->
-      phoas_expr_equiv C (PhEIf e1 e2 e3) (PhEIf e1' e2' e3')
-    | eq_PhELet C {t1 t2} (x x' : string) e1 e1' (fn_e2 : V t1 -> phoas_expr V t2) fn_e2' :
-      phoas_expr_equiv C e1 e1' ->
-      (forall v v', phoas_expr_equiv (vars _ (v, v') :: C) (fn_e2 v) (fn_e2' v')) ->
-      phoas_expr_equiv C (PhELet x e1 fn_e2) (PhELet x' e1' fn_e2').
-  End expr_equiv.
-
-  Section WithPhoasTypeEnv.
-    Context {V : type -> Type}.
-    (* Typing environment for mutable variables *)
-    Context {tenv_mut : map.map string type} {tenv_mut_ok : map.ok tenv_mut}.
-
-    Inductive phoas_wf {V : type -> Type} : tenv_mut -> forall {t : type}, phoas_expr V t -> Prop :=
-    | wf_PhEVar G t v : phoas_wf G (PhEVar t v)
-    | wf_PhELoc G t x :
-      map.get G x = Some t ->
-      phoas_wf G (PhELoc t x)
-    | wf_PhEAtom G {t} (a : atom t) : phoas_wf G (PhEAtom a)
-    | wf_PhEUnop G {t1 t2} (o : unop t1 t2) e :
-      phoas_wf G e ->
-      phoas_wf G (PhEUnop o e)
-    | wf_PhEBinop G {t1 t2 t3} (o : binop t1 t2 t3) e1 e2 :
-      phoas_wf G e1 ->
-      phoas_wf G e2 ->
-      phoas_wf G (PhEBinop o e1 e2)
-    | wf_PhEFlatmap G {t1 t2} l1 x (fn_l2 : V t1 -> phoas_expr V (TList t2)) :
-      phoas_wf G l1 ->
-      (forall v, phoas_wf G (fn_l2 v)) ->
-      phoas_wf G (PhEFlatmap l1 x fn_l2)
-    | wf_PhEFold G {t1 t2} l1 e2 x y (fn_e3 : V t1 -> V t2 -> phoas_expr V t2) :
-      phoas_wf G l1 ->
-      phoas_wf G e2 ->
-      (forall v1 v2, phoas_wf G (fn_e3 v1 v2)) ->
-      phoas_wf G (PhEFold l1 e2 x y fn_e3)
-    | wf_PhEIf G {t} e1 (e2 e3 : phoas_expr V t) :
-      phoas_wf G e1 ->
-      phoas_wf G e2 ->
-      phoas_wf G e3 ->
-      phoas_wf G (PhEIf e1 e2 e3)
-    | wf_PhELet G {t1 t2} x e1 (fn_e2 : V t1 -> phoas_expr V t2) :
-      phoas_wf G e1 ->
-      (forall v, phoas_wf G (fn_e2 v)) ->
-      phoas_wf G (PhELet x e1 fn_e2).
-
-    Definition projT1_snd_T2 {A : Type} {P1 P2 : A -> Type} (v : {t : A & (P1 t * P2 t)%type}) :
-      {t : A & P2 t} :=
-      existT _ (projT1 v) (snd (projT2 v)).
-
-    Definition dephoasify_envs_consistent (C : ctxt) (G : tenv_mut) (store l : locals) (used : list string) :=
-      (forall (p : {t : type & (string * interp_type t)%type}),
-          In p C ->
-          let s := fst (projT2 p) in
-          In s used /\
-            (* Immutable variable name not used as mutable variable *)
-            match map.get G s with
-            | Some _ => False
-            | None => True
-            end /\
-            match map.get l s with
-            | Some p' => projT1_snd_T2 p = p'
-            | None => False
-            end)
-      /\ (forall s, match map.get G s with
-                    | Some t => In s used /\
-                                  match map.get store s with
-                                  | Some p => projT1 p = t /\ map.get l s = Some p
-                                  | None => False
-                                  end
-                    | None => True
-                    end).
-
-    Lemma dephoasify_envs_consistent_immut_step: forall C G store l used t x y,
-        dephoasify_envs_consistent C G store l used ->
-        ~ In x used ->
-        dephoasify_envs_consistent (vars t (x, y) :: C) G store (set_local l x y) (x :: used).
-    Proof.
-      intros C G store l used t x y [HL HR] H_not_in. split.
-      - intros p [H_inL | H_inR].
-        + subst; simpl. unfold set_local. rewrite map.get_put_same.
-          unfold projT1_snd_T2. simpl. split;
-            [left | split]; try reflexivity.
-          pose proof (HR x) as HRx. destruct (map.get G x); trivial.
-          destruct HRx as [HRL _]. apply H_not_in. assumption.
-        + apply HL in H_inR. remember (fst (projT2 p)) as s; simpl.
-          unfold set_local. destruct H_inR. split; [right; assumption |].
-          rewrite map.get_put_diff; [assumption | congruence].
-      - intro s. pose proof (HR s) as HRs. destruct (map.get store s) eqn:E.
-        + unfold set_local. destruct (map.get G s); trivial. destruct HRs; split.
-          * right; assumption.
-          * rewrite map.get_put_diff; [assumption | congruence].
-        + destruct (map.get G s); [destruct HRs; exfalso; assumption | trivial].
-    Qed.
-
-    Lemma dephoasify_envs_consistent_used_step: forall C G store l used x,
-        dephoasify_envs_consistent C G store l used ->
-        dephoasify_envs_consistent C G store l (x::used).
-    Proof.
-      intros C G store l used x [HL HR]. simpl in *.
-      unfold dephoasify_envs_consistent. split.
-      - intros p H. pose proof (HL p H) as [HL1 [HL2 HL3]].
-        split; [right | split]; assumption.
-      - intro s. pose proof (HR s) as HR'.
-        destruct (map.get G s); destruct HR'; trivial.
-        split; [right | ]; assumption.
-    Qed.
-
-    Lemma dephoasify_sound' :
-      forall {t : type} (e : phoas_expr const_string t) (e0 : phoas_expr interp_type t) (C : ctxt),
-        phoas_expr_equiv C e e0 ->
-        forall (G : tenv_mut),
-          phoas_wf G e ->
-          forall (store l : locals) (used : list string),
-            dephoasify_envs_consistent C G store l used ->
-            interp_phoas_expr store e0 = interp_expr l (dephoasify used e).
-    Proof.
-      induction e; intros e0 C H_equiv G H_wf store l used H_consistent; simpl;
-        inversion H_equiv; inversion H_wf; subst; repeat eq_projT2_eq; simpl.
-      - unfold get_local. apply H_consistent in H3 as [_ [_ H3]]. simpl in H3.
-        destruct (map.get l v).
-        + unfold proj_expected. subst. simpl. rewrite (eq_dec_refl type_eq_dec). reflexivity.
-        + exfalso; assumption.
-      - inversion H_wf. subst. destruct H_consistent as [_ HR]. unfold get_local.
-        pose proof (HR x') as HR'. rewrite H2 in HR'; destruct HR' as [_ HR'].
-        destruct (map.get store x') eqn:E.
-        + destruct (map.get l x'); destruct HR' as [HR'L HR'R];
-            [injection HR'R as HR'R; congruence | discriminate].
-        + exfalso; assumption.
-      - f_equal; eauto.
-      - f_equal; eauto.
-      - f_equal.
-        + extensionality y. eapply H.
-          * apply H8.
-          * apply H16.
-          * apply dephoasify_envs_consistent_immut_step;
-              [assumption | apply fresh_is_fresh].
-        + eapply IHe.
-          * apply H4.
-          * apply H13.
-          * apply dephoasify_envs_consistent_used_step. assumption.
-      - f_equal; eauto.
-        extensionality v. extensionality acc.
-        eapply H; try eauto.
-        repeat apply dephoasify_envs_consistent_immut_step;
-          try apply fresh_is_fresh. assumption.
-      - erewrite IHe1 by eauto. erewrite IHe2 by eauto. erewrite IHe3 by eauto.
-        reflexivity.
-      - eapply H; eauto. erewrite IHe by eauto.
-        apply dephoasify_envs_consistent_immut_step;
-          [assumption | apply fresh_is_fresh].
-    Qed.
-
-    Definition Dephoasify (used : list string) {t : type} (e : Phoas_expr t) : expr t :=
-      dephoasify used (e const_string).
-
-    Definition dephoasify_envs_consistent_closed (G : tenv_mut) (store l : locals) (used : list string) : Prop :=
-      forall s : string, match map.get G s with
-                         | Some t => In s used /\
-                                       match map.get store s with
-                                       | Some p => projT1 p = t /\ map.get l s = Some p
-                                       | None => False
-                                       end
-                         | None => True
-                         end.
-
-    Definition Phoas_wf (G : tenv_mut) {t : type} (e : Phoas_expr t) :=
-      (forall V1 V2, phoas_expr_equiv nil (e V1) (e V2)) /\
-        forall V, phoas_wf G (e V).
-
-    Theorem dephoasify_sound : forall {t : type} (e : Phoas_expr t) (G : tenv_mut) ,
-        Phoas_wf G e ->
-        forall (store l : locals) (used : list string),
-          dephoasify_envs_consistent_closed G store l used ->
-          interp_phoas_expr store (e interp_type) = interp_expr l (Dephoasify used e).
-    Proof.
-      intros t e G [H_equiv H_wf] store l used H_consistent_closed.
-      eapply dephoasify_sound'.
-      - apply H_equiv.
-      - apply H_wf.
-      - unfold dephoasify_envs_consistent. split.
-        + intros p contra. apply in_nil in contra. exfalso; assumption.
-        + assumption.
-    Qed.
-
-  End WithPhoasTypeEnv.
+  Definition Phoasify {t : type} (e : expr t) : Phoas_expr t:=
+    fun (V : type -> Type) => phoasify (V := V) map.empty e.
 End WithMap.
 
+Definition Phoas_wf {t : type} (e : Phoas_expr t) :=
+  forall V1 V2, phoas_expr_equiv nil (e V1) (e V2).
 
-(* TODO: move eq_dec_refl elsewhere
-Flat_wf to Phoas_wf and vice versa
-Try out separated tenv into mut and immut? By an auxiliary file instead of refactoring?
-mem for bare metal; store for mutable; env for immutable *)
+(* Remove one occurrence of x from store if there is one.
+ * Auxiliary function for the definition of fresh' below *)
+Fixpoint remove_one (x : string) (l : list string) : list string :=
+  match l with
+  | nil => nil
+  | h :: t => if eqb h x then t else h :: remove_one x t
+  end.
+
+Lemma in_remove_one_len : forall (x : string) (l : list string),
+    In x l -> List.length l = S (List.length (remove_one x l)).
+Proof.
+  intros. induction l.
+  - apply in_nil in H. exfalso. apply H.
+  - simpl in H. destruct (eqb a x) eqn:E.
+    + simpl. rewrite E. reflexivity.
+    + destruct H as [HL | HR].
+      * rewrite <- eqb_eq in HL. rewrite HL in E. discriminate.
+      * simpl. rewrite E. simpl. rewrite (IHl HR). reflexivity.
+Qed.
+
+Lemma in_remove_one : forall (x : string) (l : list string),
+    In x l -> forall (y : string), x = y \/ In x (remove_one y l).
+Proof.
+  intros x l H. induction l.
+  - intros. apply in_nil in H. exfalso. exact H.
+  - intros y. simpl in H. destruct H as [HL | HR].
+    + destruct (eqb a y) eqn:E.
+      * rewrite eqb_eq in E. rewrite HL in E. left. exact E.
+      * right. simpl. rewrite E. simpl. left. exact HL.
+    + destruct (IHl HR) with (y := y) as [HL' | HR'].
+      * left. exact HL'.
+      * right. simpl. destruct (eqb a y) eqn:E.
+        { exact HR. }
+        { simpl. right. exact HR'. }
+Qed.
+
+(* Append "'"s to x until the resulting name is not in used.
+ * The initial call should have (budget = length used) *)
+Fixpoint fresh' (budget : nat) (used : list string) (x : string) : string :=
+  (* We need budget as a decreasing argument for the function *)
+  match budget with
+  | O => x
+  | S n => match in_dec string_dec x used with
+           | left _ => fresh' n (remove_one x used) (x ++ "'")
+           | right _ => x
+           end
+  end.
+
+(* Given a list of used names and a hint, return a fresh name *)
+Definition fresh (used : list string) (x : string) : string :=
+  fresh' (List.length used) used x.
+
+Lemma len_app : forall y, length y < length (y ++ "'").
+Proof.
+  induction y; auto. simpl. apply Arith_prebase.lt_n_S_stt. apply IHy.
+Qed.
+
+Lemma fresh'_len : forall (budget : nat) (used : list string) (x : string),
+    length x <= length (fresh' budget used x).
+Proof.
+  induction budget; intros.
+  - destruct used; unfold fresh'; constructor.
+  - destruct (in_dec string_dec x used) eqn:E.
+    + unfold fresh'. rewrite E.
+      apply Nat.le_trans with (m := length (x ++ "'")).
+      * pose proof (len_app x) as len_app_x.
+        apply Nat.lt_le_incl. exact len_app_x.
+      * apply (IHbudget (remove_one x used) (x ++ "'")%string).
+    + unfold fresh'; rewrite E; constructor.
+Qed.
+
+Lemma fresh'_is_fresh : forall (budget : nat) (used : list string) (x : string),
+    budget = List.length used -> ~ In (fresh' budget used x) used.
+Proof.
+  induction budget; intros.
+  - destruct used.
+    + auto.
+    + discriminate.
+  - rewrite H. destruct (in_dec string_dec x used) as [ HL | HR ] eqn:E.
+    + assert (Hrm_len: S budget = S (List.length (remove_one x used))).
+      { rewrite H. apply in_remove_one_len. apply HL. }
+      injection Hrm_len as Hrm_len.
+      apply (IHbudget (remove_one x used)) with (x := (x ++ "'")%string) in Hrm_len as Hrm.
+      unfold not. intros. apply in_remove_one with (y := x) in H0 as [HL'|HR'].
+      * assert (HA : length (x ++ "'") <= length (fresh' (Datatypes.length used) used x)).
+        { unfold fresh'. rewrite <- H. rewrite E. apply fresh'_len. }
+        rewrite HL' in HA. apply Arith_prebase.le_not_lt_stt in HA.
+        apply HA. apply len_app.
+      * unfold fresh' in HR'. rewrite <- H in HR'. rewrite E in HR'.
+        apply Hrm. unfold fresh'. apply HR'.
+    + unfold fresh'. rewrite <- H. rewrite E. exact HR.
+Qed.
+
+Corollary fresh_is_fresh : forall (used : list string) (x : string), ~ In (fresh used x) used.
+Proof.
+  intros. unfold fresh. apply fresh'_is_fresh. reflexivity.
+Qed.
+
+Definition const_string : type -> Type := fun _ => string.
+
+Fixpoint dephoasify (used : list string) {t : type} (e : phoas_expr const_string t) : expr t :=
+  match e with
+  | PhEVar _ v => EVar _ v
+  | PhELoc _ x => ELoc _ x
+  | PhEAtom a => EAtom a
+  | PhEUnop o e1 => EUnop o (dephoasify used e1)
+  | PhEBinop o e1 e2 => EBinop o (dephoasify used e1) (dephoasify used e2)
+  | PhEFlatmap l1 x fn =>
+      let x' := fresh used x in
+      let used' := x' :: used in
+      EFlatmap (dephoasify used l1) x' (dephoasify used' (fn x'))
+  | PhEIf e1 e2 e3 => EIf (dephoasify used e1) (dephoasify used e2) (dephoasify used e3)
+  | PhEFold l1 a x y fn =>
+      let x' := fresh used x in
+      let y' := fresh (x' :: used) y in
+      let used' := y' :: x' :: used in
+      EFold (dephoasify used l1) (dephoasify used a) x' y' (dephoasify used' (fn x' y'))
+  | PhELet x e1 fn =>
+      let x' := fresh used x in
+      let used' := x' :: used in
+      ELet x' (dephoasify used e1) (dephoasify used' (fn x'))
+  end.
+
+Definition Dephoasify (used : list string) {t : type} (e : Phoas_expr t) : expr t :=
+  dephoasify used (e const_string).
+
+Lemma eq_dec_refl : forall  {t : Type} (eq_dec : forall (v1 v2 : t), {v1 = v2} + {v1 <> v2}),
+  forall (x : t), eq_dec x x = left eq_refl.
+Proof.
+  intros t eq_dec x. destruct (eq_dec x x).
+  - f_equal. apply Eqdep_dec.UIP_dec. apply eq_dec.
+  - exfalso. apply n. reflexivity.
+Qed.
+
+Ltac eq_projT2_eq := match goal with
+                     | H : existT ?f ?t _ = existT ?f ?t _ |- _ =>
+                         apply Eqdep_dec.inj_pair2_eq_dec in H;[ subst; eauto | apply type_eq_dec]
+                     end.
+
+(*??? move to util?*)
+Lemma fold_right_ext : forall (A B : Type) (f g : B -> A -> A) (a : A) (l : list B),
+    (forall x y, f x y = g x y) ->
+    fold_right f a l = fold_right g a l.
+Proof.
+  induction l as [|a' l' IHl] ; intro H.
+  - reflexivity.
+  - simpl. rewrite (IHl H). apply H.
+Qed.
+
+Section WithMap.
+  Context {width: Z} {BW: Bitwidth width} {word: word.word width} {mem: map.map word byte}.
+  Context {word_ok: word.ok word} {mem_ok: map.ok mem}.
+  Context {phoas_env : forall V, map.map string {t : type & V t}} {phoas_env_ok : forall V, map.ok (phoas_env V)}.
+
+  Lemma default_val_eq : forall store t,
+      interp_phoas_expr store (default_phoas_expr t) = default_val t.
+  Proof.
+    induction t; try reflexivity.
+    (* TPair *)
+    simpl. rewrite IHt1, IHt2. reflexivity.
+  Qed.
+
+  Lemma proj_expected_eq : forall store t v,
+      interp_phoas_expr store (phoas_proj_expected t v) = proj_expected t v.
+  Proof.
+    intros store t v.
+    unfold phoas_proj_expected. unfold proj_expected.
+    destruct (type_eq_dec (projT1 v) t).
+    - reflexivity.
+    - apply default_val_eq.
+  Qed.
+
+  Lemma phoasify_sound' :
+    forall {t : type} (e : expr t) (store env : phoas_env interp_type),
+      interp_expr store env e = interp_phoas_expr store (phoasify env e).
+  Proof.
+    induction e; intros store env; simpl; try reflexivity.
+    - unfold get_local. destruct (map.get env x) eqn:E.
+      + symmetry. apply proj_expected_eq.
+      + symmetry. apply default_val_eq.
+    - rewrite IHe. reflexivity.
+    - rewrite IHe1, IHe2; reflexivity.
+    - rewrite IHe1. apply flat_map_ext.
+      intro; rewrite IHe2; reflexivity.
+    - rewrite IHe1, IHe2. apply fold_right_ext.
+      intros; rewrite IHe3; reflexivity.
+    - rewrite IHe1, IHe2, IHe3; reflexivity.
+    - rewrite IHe1, IHe2; reflexivity.
+  Qed.
+
+  Theorem phoasify_sound : forall (store : phoas_env interp_type) {t : type} (e : expr t),
+      interp_expr store map.empty e = interp_Phoas_expr store (Phoasify e).
+  Proof.
+    intros store t e. unfold Phoasify. unfold interp_Phoas_expr.
+    apply phoasify_sound'.
+  Qed.
+
+  Definition phoasify_form_consistent {V V'} (C : @ctxt V V')
+    (env : phoas_env V) (env' : phoas_env V') :=
+    forall x, match map.get env x with
+              | Some v => match map.get env' x with
+                          | Some v' => exists p,
+                              In p C /\
+                                projT1_fst_T2 p = v /\
+                                projT1_snd_T2 p = v'
+                          | None => False
+                          end
+              | None => map.get env' x = None
+              end.
+
+  Lemma phoasify_form_consistent_step : forall V V' (C : @ctxt V V') env env',
+      phoasify_form_consistent C env env' ->
+      forall y t (u : V t) (u' : V' t),
+        phoasify_form_consistent (vars _ (u, u') :: C) (set_phoas_local env y u) (set_phoas_local env' y u').
+  Proof.
+    unfold phoasify_form_consistent.
+    intros V V' C env env' H y t u u' x.
+    unfold set_phoas_local. destruct (eqb x y) eqn:E.
+    - rewrite eqb_eq in E. rewrite E.
+      repeat rewrite map.get_put_same.
+      exists (vars t (u, u')). split.
+      + left; reflexivity.
+      + split; reflexivity.
+    - rewrite eqb_neq in E. repeat rewrite map.get_put_diff; try assumption.
+      pose proof (H x) as H. destruct (map.get env x).
+      + destruct (map.get env' x); [| exfalso; assumption].
+        destruct H as [p [H1 H2]].
+        exists p. split; [right |]; assumption.
+      + assumption.
+  Qed.
+
+  Lemma phoas_equiv_default : forall V V' (C : @ctxt V V') (t : type),
+      phoas_expr_equiv C (default_phoas_expr t) (default_phoas_expr t).
+  Proof.
+    induction t; constructor; try reflexivity.
+    (* TPair *)
+    ++ apply IHt1.
+    ++ apply IHt2.
+  Qed.
+
+  Lemma phoasify_wf' : forall V V' (C : @ctxt V V') (env : phoas_env V) (env' : phoas_env V'),
+      phoasify_form_consistent C env env' ->
+      forall t (e : expr t) ,
+        phoas_expr_equiv C (phoasify env e) (phoasify env' e).
+  Proof.
+    intros V V' C env env' H_consistent t e.
+    generalize dependent env'; generalize dependent env; generalize dependent C.
+    induction e; intros C env env' H_consistent.
+    - simpl. pose proof (H_consistent x) as H.
+      destruct (map.get env x).
+      + destruct (map.get env' x); try (exfalso; assumption).
+        * unfold phoas_proj_expected. destruct s; destruct s0; simpl.
+          destruct H as [[t' [l r]] [H1 [H2 H3]]].
+          unfold projT1_fst_T2 in H2; unfold projT1_snd_T2 in H3; simpl in *.
+          apply projT1_eq in H2 as H2'. apply projT1_eq in H3 as H3'.
+          simpl in H2', H3'. subst. repeat eq_projT2_eq.
+          destruct (type_eq_dec x1 t).
+          -- constructor. subst. assumption.
+          -- apply phoas_equiv_default.
+      + rewrite H. apply phoas_equiv_default.
+    - constructor; reflexivity.
+    - constructor; reflexivity.
+    - constructor; apply IHe, H_consistent.
+    - constructor; [apply IHe1 | apply IHe2]; apply H_consistent.
+    - constructor.
+      + apply IHe1, H_consistent.
+      + intros v v'. apply IHe2.
+        apply phoasify_form_consistent_step, H_consistent.
+    - constructor.
+      + apply IHe1, H_consistent.
+      + apply IHe2, H_consistent.
+      + intros v1 v2 v1' v2'. apply IHe3.
+        repeat apply phoasify_form_consistent_step. apply H_consistent.
+    - constructor; [apply IHe1 | apply IHe2 | apply IHe3]; apply H_consistent.
+    - constructor.
+      + apply IHe1, H_consistent.
+      + intros v v'. apply IHe2.
+        apply phoasify_form_consistent_step, H_consistent.
+  Qed.
+
+  Theorem phoasify_wf : forall t (e : expr t),
+      Phoas_wf (Phoasify e).
+  Proof.
+    unfold Phoas_wf. unfold Phoasify. intros t e V V'.
+    apply phoasify_wf'. unfold phoasify_form_consistent.
+    intro x. repeat rewrite map.get_empty. reflexivity.
+  Qed.
+
+
+  Definition dephoasify_envs_consistent (C : ctxt) (used : list string) (env : phoas_env interp_type) :=
+    forall (p : {t : type & (string * interp_type t)%type}),
+      In p C ->
+      let s := fst (projT2 p) in
+      In s used /\ map.get env s = Some (projT1_snd_T2 p).
+
+  Lemma dephoasify_envs_consistent_step : forall C used env,
+      dephoasify_envs_consistent C used env ->
+      forall x t (v : interp_type t),
+        dephoasify_envs_consistent (vars _ (fresh used x, v) :: C) (fresh used x :: used) (set_local env (fresh used x) v).
+  Proof.
+    unfold dephoasify_envs_consistent. intros C used env H x t v p [HL | HR].
+    - rewrite <- HL. split.
+      + left; reflexivity.
+      + simpl. unfold set_local. rewrite map.get_put_same. reflexivity.
+    - apply H in HR as [HRL HRR]. split.
+      + right; apply HRL.
+      + unfold set_local. destruct (eqb (fst (projT2 p)) (fresh used x)) eqn:E.
+        * rewrite eqb_eq in E. rewrite E in HRL. apply fresh_is_fresh in HRL.
+          exfalso; assumption.
+        * rewrite eqb_neq in E. rewrite map.get_put_diff; assumption.
+  Qed.
+
+  Lemma dephoasify_sound' :
+    forall (t : type) (e : phoas_expr const_string t) (e0 : phoas_expr interp_type t) (C : ctxt),
+      phoas_expr_equiv C e e0 ->
+      forall (used : list string) (env : phoas_env interp_type),
+        dephoasify_envs_consistent C used env ->
+        forall (store : phoas_env interp_type),
+          interp_phoas_expr store e0 = interp_expr store env (dephoasify used e).
+  Proof.
+    intros t e e0 C H_equiv. induction H_equiv; intros used env H_consistent store; simpl.
+    - unfold dephoasify_envs_consistent in H_consistent.
+      apply H_consistent in H. destruct H as [_ HR].
+      simpl in HR. unfold get_local. destruct (map.get env v).
+      + unfold projT1_snd_T2 in HR. simpl in HR.
+        unfold proj_expected. injection HR as HR. rewrite HR.
+        simpl. rewrite eq_dec_refl. reflexivity.
+      + discriminate.
+    - rewrite H; reflexivity.
+    - rewrite H; reflexivity.
+    - f_equal. apply IHH_equiv. apply H_consistent.
+    - f_equal.
+      + apply IHH_equiv1. apply H_consistent.
+      + apply IHH_equiv2. apply H_consistent.
+    - rewrite (IHH_equiv _ _ H_consistent). apply flat_map_ext.
+      remember (fresh used x) as y.
+      intros v'. rewrite H0 with (v := y) (used := y :: used) (env := set_local env y v').
+      + reflexivity.
+      + rewrite Heqy. apply dephoasify_envs_consistent_step. apply H_consistent.
+    - rewrite (IHH_equiv1 _ _ H_consistent), (IHH_equiv2 _ _ H_consistent).
+      apply fold_right_ext. intros v1 v2. apply H0.
+      repeat apply dephoasify_envs_consistent_step. apply H_consistent.
+    - rewrite (IHH_equiv1 _ _ H_consistent), (IHH_equiv2 _ _ H_consistent), (IHH_equiv3 _ _ H_consistent). reflexivity.
+    - rewrite (IHH_equiv _ _ H_consistent). remember (fresh used x) as y.
+      remember (interp_expr store env (dephoasify used e1)) as v.
+      rewrite H0 with (v := y) (used := y :: used) (env := set_local env y v);
+        [reflexivity |].
+      rewrite Heqy. apply dephoasify_envs_consistent_step. apply H_consistent.
+  Qed.
+
+  Theorem dephoasify_sound : forall {t : type} (e : Phoas_expr t),
+      Phoas_wf e ->
+      forall (store : phoas_env interp_type) (used : list string),
+        interp_phoas_expr store (e interp_type) = interp_expr store map.empty (Dephoasify used e).
+  Proof.
+    intros t e H_wf store used.
+    apply dephoasify_sound' with (C := nil) (env := map.empty).
+    - apply H_wf.
+    - unfold dephoasify_envs_consistent. intros p contra.
+      apply in_nil in contra. exfalso; assumption.
+  Qed.
+End WithMap.
